parse32, serialize32 bounded int32

src/lowparse/LowParse.SLow.BoundedInt.fsti
@@ -103,3 +103,74 @@ let size32_u32_le: size32 serialize_u32_le =
   assert_norm (size32_constant_precond serialize_u32_le 4ul);
   size32_constant serialize_u32_le 4ul ()
 
+module U32 = FStar.UInt32
+
+val parse32_bounded_int32_1
+  (min32: U32.t)
+  (max32: U32.t { 0 < U32.v max32 /\ U32.v min32 <= U32.v max32 /\ U32.v max32 < 256 })
+: Tot (parser32 (parse_bounded_int32 (U32.v min32) (U32.v max32)))
+
+val parse32_bounded_int32_2
+  (min32: U32.t)
+  (max32: U32.t { 256 <= U32.v max32 /\ U32.v min32 <= U32.v max32 /\ U32.v max32 < 65536 })
+: Tot (parser32 (parse_bounded_int32 (U32.v min32) (U32.v max32)))
+
+val parse32_bounded_int32_3
+  (min32: U32.t)
+  (max32: U32.t { 65536 <= U32.v max32 /\ U32.v min32 <= U32.v max32 /\ U32.v max32 < 16777216 })
+: Tot (parser32 (parse_bounded_int32 (U32.v min32) (U32.v max32)))
+
+val parse32_bounded_int32_4
+  (min32: U32.t)
+  (max32: U32.t { 16777216 <= U32.v max32 /\ U32.v min32 <= U32.v max32 /\ U32.v max32 < 4294967296 })
+: Tot (parser32 (parse_bounded_int32 (U32.v min32) (U32.v max32)))
+
+inline_for_extraction
+let parse32_bounded_int32
+  (min32: U32.t)
+  (max32: U32.t { 0 < U32.v max32 /\ U32.v min32 <= U32.v max32 /\ U32.v max32 < 4294967296 })
+: Tot (parser32 (parse_bounded_int32 (U32.v min32) (U32.v max32)))
+= fun input -> (
+  if max32 `U32.lt` 256ul
+  then parse32_bounded_int32_1 min32 max32 input
+  else if max32 `U32.lt` 65536ul
+  then parse32_bounded_int32_2 min32 max32 input
+  else if max32 `U32.lt` 16777216ul
+  then parse32_bounded_int32_3 min32 max32 input
+  else parse32_bounded_int32_4 min32 max32 input
+  )
+
+val serialize32_bounded_int32_1
+  (min32: U32.t)
+  (max32: U32.t { 0 < U32.v max32 /\ U32.v min32 <= U32.v max32 /\ U32.v max32 < 256 })
+: Tot (serializer32 (serialize_bounded_int32 (U32.v min32) (U32.v max32)))
+
+val serialize32_bounded_int32_2
+  (min32: U32.t)
+  (max32: U32.t { 256 <= U32.v max32 /\ U32.v min32 <= U32.v max32 /\ U32.v max32 < 65536 })
+: Tot (serializer32 (serialize_bounded_int32 (U32.v min32) (U32.v max32)))
+
+val serialize32_bounded_int32_3
+  (min32: U32.t)
+  (max32: U32.t { 65536 <= U32.v max32 /\ U32.v min32 <= U32.v max32 /\ U32.v max32 < 16777216 })
+: Tot (serializer32 (serialize_bounded_int32 (U32.v min32) (U32.v max32)))
+
+val serialize32_bounded_int32_4
+  (min32: U32.t)
+  (max32: U32.t { 16777216 <= U32.v max32 /\ U32.v min32 <= U32.v max32 /\ U32.v max32 < 4294967296 })
+: Tot (serializer32 (serialize_bounded_int32 (U32.v min32) (U32.v max32)))
+
+inline_for_extraction
+let serialize32_bounded_int32
+  (min32: U32.t)
+  (max32: U32.t { 0 < U32.v max32 /\ U32.v min32 <= U32.v max32 /\ U32.v max32 < 4294967296 })
+: Tot (serializer32 (serialize_bounded_int32 (U32.v min32) (U32.v max32)))
+= fun input -> (
+  if max32 `U32.lt` 256ul
+  then serialize32_bounded_int32_1 min32 max32 input
+  else if max32 `U32.lt` 65536ul
+  then serialize32_bounded_int32_2 min32 max32 input
+  else if max32 `U32.lt` 16777216ul
+  then serialize32_bounded_int32_3 min32 max32 input
+  else serialize32_bounded_int32_4 min32 max32 input
+  )
